LocallyNameless/STLC.v
@@ -3,8 +3,10 @@ From FormalSystems Require Export LocallyNameless.LocallyNameless.
 (** * Types *)
 
 Inductive Ty : Type :=
+| TyFun  : Ty -> Ty -> Ty
 | TyUnit : Ty
-| TyFun  : Ty -> Ty -> Ty.
+| TyEmpty : Ty
+| TyProd : Ty -> Ty -> Ty.
 
 Fixpoint eq_dec_Ty (A B : Ty) : {A = B} + {A <> B}.
 Proof.
@@ -28,9 +30,16 @@ Defined.
 
 Inductive Tm : Type :=
 | fvar (a : Atom) : Tm
-| bvar : nat -> Tm
-| abs  : Tm -> Tm
-| app  : Tm -> Tm -> Tm.
+| bvar  : nat -> Tm
+| abs   : Tm -> Tm
+| app   : Tm -> Tm -> Tm
+| unit  : Tm
+| elimUnit : Tm -> Tm -> Tm
+| elimUnit' : Tm -> Tm -> Tm
+| abort : Tm -> Tm
+| pair  : Tm -> Tm -> Tm
+| outl  : Tm -> Tm
+| outr  : Tm -> Tm.
 
 Coercion fvar : Atom >-> Tm.
 Coercion bvar : nat >-> Tm.
@@ -38,8 +47,8 @@ Coercion bvar : nat >-> Tm.
 Fixpoint eq_dec_Tm (t u : Tm) : {t = u} + {t <> u}.
 Proof.
   decide equality.
-  - apply eq_dec_Atom.
-  - decide equality.
+  - apply (eq_dec_Atom a a0).
+  - apply PeanoNat.Nat.eq_dec.
 Defined.
 
 #[export, refine] Instance Decidable_eq_Tm :
@@ -60,26 +69,52 @@ Defined.
 #[export] Instance Open_Tm : Open nat Atom Tm :=
   fix open (t : Tm) (i : nat) (a : Atom) : Tm :=
     match t with
-    | fvar a    => fvar a
-    | bvar j    => if decide (i = j) then a else bvar j
-    | abs t'    => abs (open t' (S i) a)
-    | app t1 t2 => app (open t1 i a) (open t2 i a)
+    | fvar a     => fvar a
+    | bvar j     => if decide (i = j) then a else bvar j
+    | abs t'     => abs (open t' (S i) a)
+    | app t1 t2  => app (open t1 i a) (open t2 i a)
+    | unit       => unit
+    | elimUnit t1 t2 => elimUnit (open t1 i a) (open t2 (S i) a)
+    | elimUnit' t1 t2 => elimUnit' (open t1 i a) (open t2 i a)
+    | abort t'   => abort (open t' i a)
+    | pair t1 t2 => pair (open t1 i a) (open t2 i a)
+    | outl t'    => outl (open t' i a)
+    | outr t'    => outr (open t' i a)
     end.
 
 #[export] Instance Close_Tm : Close nat Atom Tm :=
   fix close (t : Tm) (i : nat) (a : Atom) : Tm :=
     match t with
-    | fvar x    => if decide (a = x) then bvar i else fvar x
-    | bvar n    => bvar n
-    | abs t'    => abs (close t' (S i) a)
-    | app t1 t2 => app (close t1 i a) (close t2 i a)
+    | fvar x     => if decide (a = x) then bvar i else fvar x
+    | bvar n     => bvar n
+    | abs t'     => abs (close t' (S i) a)
+    | app t1 t2  => app (close t1 i a) (close t2 i a)
+    | unit       => unit
+    | elimUnit t1 t2 => elimUnit (close t1 i a) (close t2 (S i) a)
+    | elimUnit' t1 t2 => elimUnit' (close t1 i a) (close t2 i a)
+    | abort t'   => abort (close t' i a)
+    | pair t1 t2 => pair (close t1 i a) (close t2 i a)
+    | outl t'    => outl (close t' i a)
+    | outr t'    => outr (close t' i a)
     end.
 
 #[export, refine] Instance OC_Tm :
   OC nat Atom Tm Open_Tm Close_Tm := {}.
 Proof.
   all: induction t; cbn; intros;
-    [now decide_all | now decide_all | now rewrite IHt; congruence | now rewrite IHt1, IHt2].
+  [
+    now decide_all                     |
+    now decide_all                     |
+    now rewrite IHt; congruence        |
+    now rewrite IHt1, IHt2             |
+    easy                               |
+    now rewrite IHt1, IHt2; congruence |
+    now rewrite IHt1, IHt2             |
+    now rewrite IHt                    |
+    now rewrite IHt1, IHt2             |
+    now rewrite IHt                    |
+    now rewrite IHt
+  ].
 Qed.
 
 Lemma open_open :
@@ -93,36 +128,56 @@ Proof.
   - now decide_all.
   - inversion H.
     f_equal.
-    now eapply IHt, H1; lia.
+    now apply IHt in H1; [| lia].
   - inversion H.
     f_equal.
     + now apply IHt1 in H1.
     + now apply IHt2 in H2.
+  - easy.
+  - inversion H.
+    f_equal.
+    + now apply IHt1 in H1.
+    + now apply IHt2 in H2; [| lia].
+  - inversion H.
+    f_equal.
+    + now apply IHt1 in H1.
+    + now apply IHt2 in H2; [| lia].
+  - inversion H.
+    f_equal.
+    now apply IHt in H1.
+  - inversion H.
+    f_equal.
+    + now apply IHt1 in H1.
+    + now apply IHt2 in H2.
+  - inversion H.
+    f_equal.
+    now apply IHt in H1; [| lia].
+  - inversion H.
+    f_equal.
+    now apply IHt in H1; [| lia].
 Qed.
 
 (** ** Locally nameless *)
 
 Fixpoint fv (t : Tm) : list Atom :=
 match t with
-| fvar x    => [x]
-| bvar _    => []
-| abs t'    => fv t'
-| app t1 t2 => fv t1 ++ fv t2
+| fvar x     => [x]
+| bvar _     => []
+| abs t'     => fv t'
+| app t1 t2  => fv t1 ++ fv t2
+| unit       => []
+| elimUnit t1 t2 => fv t1 ++ fv t2
+| elimUnit' t1 t2 => fv t1 ++ fv t2
+| abort t'   => fv t'
+| pair t1 t2 => fv t1 ++ fv t2
+| outl t'    => fv t'
+| outr t'    => fv t'
 end.
 
 #[export, refine] Instance LocallyNameless_Tm :
   LocallyNameless Atom Tm Open_Tm Close_Tm OC_Tm :=
 {
   fv := fv;
-(*
-    fix fv (t : Tm) : list Atom :=
-    match t with
-    | fvar x    => [x]
-    | bvar _    => []
-    | abs t'    => fv t'
-    | app t1 t2 => fv t1 ++ fv t2
-    end;
-*)
 }.
 Proof.
   - unfold supports, Fresh'.
@@ -134,16 +189,34 @@ Proof.
       now apply Fresh'_invariant, IHt.
     + intros a Hfresh.
       now rewrite IHt1, IHt2; only 2-3: solve_fresh.
+    + easy.
+    + intros a Hfresh.
+      f_equal.
+      * now rewrite IHt1 by solve_fresh.
+      * now rewrite close_invariant, IHt2 by solve_fresh.
+    + intros a Hfresh.
+      now rewrite IHt1, IHt2; only 2-3: solve_fresh.
+    + intros a Hfresh.
+      f_equal.
+      now apply Fresh'_invariant, IHt.
+    + intros a Hfresh.
+      now rewrite IHt1, IHt2; only 2-3: solve_fresh.
+    + intros a Hfresh.
+      f_equal.
+      now apply Fresh'_invariant, IHt.
+    + intros a Hfresh.
+      f_equal.
+      now apply Fresh'_invariant, IHt.
   - unfold LocallyClosed.
-    induction t as [a | i | t' | t1 IHt1 t2 IHt2]; cbn.
+    induction t; cbn.
     + exists 0.
       intros _ _.
       now exists (fresh []).
-    + exists (S i).
+    + exists (S n).
       intros j Hij.
       exists (fresh []).
       now decide_all; lia.
-    + destruct IHt' as [i IH].
+    + destruct IHt as [i IH].
       exists i.
       intros j Hij.
       destruct (IH (S j) ltac:(lia)) as [a Ha].
@@ -161,6 +234,60 @@ Proof.
         now rapply IH1.
       * rewrite (open_LocallyClosed _ i2); [easy | | now lia].
         now rapply IH2.
+    + now exists 0; intros _ _; exists (fresh []).
+    + destruct IHt1 as [i1 IH1], IHt2 as [i2 IH2].
+      exists (max i1 i2).
+      intros j Hle.
+      destruct
+        (IH1 (max i1 i2) ltac:(lia)) as [a1 Ha1],
+        (IH2 (max i1 i2) ltac:(lia)) as [a2 Ha2].
+      exists (fresh (fv t1 ++ fv t2 ++ [a1; a2])).
+      f_equal.
+      * rewrite (open_LocallyClosed _ i1); [easy | | now lia].
+        now rapply IH1.
+      * rewrite (open_LocallyClosed _ i2); [easy | | now lia].
+        now rapply IH2.
+    + destruct IHt1 as [i1 IH1], IHt2 as [i2 IH2].
+      exists (max i1 i2).
+      intros j Hle.
+      destruct
+        (IH1 (max i1 i2) ltac:(lia)) as [a1 Ha1],
+        (IH2 (max i1 i2) ltac:(lia)) as [a2 Ha2].
+      exists (fresh (fv t1 ++ fv t2 ++ [a1; a2])).
+      f_equal.
+      * rewrite (open_LocallyClosed _ i1); [easy | | now lia].
+        now rapply IH1.
+      * rewrite (open_LocallyClosed _ i2); [easy | | now lia].
+        now rapply IH2.
+    + destruct IHt as [i IH].
+      exists i; intros j Hij.
+      destruct (IH j Hij) as [a Ha].
+      exists a.
+      now rewrite Ha.
+    + destruct IHt1 as [i1 IH1], IHt2 as [i2 IH2].
+      exists (max i1 i2).
+      intros j Hle.
+      destruct
+        (IH1 (max i1 i2) ltac:(lia)) as [a1 Ha1],
+        (IH2 (max i1 i2) ltac:(lia)) as [a2 Ha2].
+      exists (fresh (fv t1 ++ fv t2 ++ [a1; a2])).
+      f_equal.
+      * rewrite (open_LocallyClosed _ i1); [easy | | now lia].
+        now rapply IH1.
+      * rewrite (open_LocallyClosed _ i2); [easy | | now lia].
+        now rapply IH2.
+    + destruct IHt as [i IH].
+      exists i.
+      intros j Hij.
+      destruct (IH j Hij) as [a Ha].
+      exists a.
+      now rewrite Ha.
+    + destruct IHt as [i IH].
+      exists i.
+      intros j Hij.
+      destruct (IH j Hij) as [a Ha].
+      exists a.
+      now rewrite Ha.
 Defined.
 
 (** ** Characterization of local closure *)
@@ -177,7 +304,34 @@ Inductive LocallyClosed' : nat -> Tm -> Prop :=
     LocallyClosed' (S i) t' -> LocallyClosed' i (abs t')
 | LocallyClosed'_app :
   forall (i : nat) (t1 t2 : Tm),
-    LocallyClosed' i t1 -> LocallyClosed' i t2 -> LocallyClosed' i (app t1 t2).
+    LocallyClosed' i t1 -> LocallyClosed' i t2 -> LocallyClosed' i (app t1 t2)
+| LocallyClosed'_unit :
+  forall i : nat,
+    LocallyClosed' i unit
+| LocallyClosed'_elimUnit :
+  forall (i : nat) (t1 t2 : Tm),
+    LocallyClosed' i t1 ->
+    LocallyClosed' (S i) t2 ->
+    LocallyClosed' i (elimUnit t1 t2)
+| LocallyClosed'_elimUnit' :
+  forall (i : nat) (t1 t2 : Tm),
+    LocallyClosed' i t1 ->
+    LocallyClosed' i t2 ->
+    LocallyClosed' i (elimUnit' t1 t2)
+| LocallyClosed'_abort :
+  forall (i : nat) (t' : Tm),
+    LocallyClosed' i t' -> LocallyClosed' i (abort t')
+| LocallyClosed'_pair :
+  forall (i : nat) (t1 t2 : Tm),
+    LocallyClosed' i t1 -> LocallyClosed' i t2 -> LocallyClosed' i (pair t1 t2)
+| LocallyClosed'_outl :
+  forall (i : nat) (t' : Tm),
+    LocallyClosed' i t' -> LocallyClosed' i (outl t')
+| LocallyClosed'_outr :
+  forall (i : nat) (t' : Tm),
+    LocallyClosed' i t' -> LocallyClosed' i (outr t').
+
+#[export] Hint Constructors LocallyClosed' : core.
 
 Lemma LocallyClosed'_spec :
   forall (i : nat) (t : Tm),
@@ -198,25 +352,88 @@ Proof.
       f_equal.
       * now rewrite open_invariant, IH1.
       * now rewrite open_invariant, IH2.
+    + now exists (fresh []).
+    + destruct
+        (IHLocallyClosed'1 j Hij) as [a1 IH1],
+        (IHLocallyClosed'2 (S j) ltac:(lia)) as [a2 IH2].
+      exists (fresh (fv t1 ++ fv t2 ++ [a1; a2])).
+      f_equal.
+      * now rewrite open_invariant, IH1.
+      * now rewrite open_invariant, IH2.
+    + destruct
+        (IHLocallyClosed'1 j Hij) as [a1 IH1],
+        (IHLocallyClosed'2 j Hij) as [a2 IH2].
+      exists (fresh (fv t1 ++ fv t2 ++ [a1; a2])).
+      f_equal.
+      * now rewrite open_invariant, IH1.
+      * now rewrite open_invariant, IH2.
+    + destruct (IHLocallyClosed' j Hij) as [a Ha].
+      now exists a; f_equal.
+    + destruct
+        (IHLocallyClosed'1 j Hij) as [a1 IH1],
+        (IHLocallyClosed'2 j Hij) as [a2 IH2].
+      exists (fresh (fv t1 ++ fv t2 ++ [a1; a2])).
+      f_equal.
+      * now rewrite open_invariant, IH1.
+      * now rewrite open_invariant, IH2.
+    + destruct (IHLocallyClosed' j Hij) as [a Ha].
+      now exists a; f_equal.
+    + destruct (IHLocallyClosed' j Hij) as [a Ha].
+      now exists a; f_equal.
   - revert i.
-    induction t as [a | n | t' IH | t1 IH1 t2 IH2]; cbn; intros i Hlc.
+    induction t; cbn; intros i Hlc.
     + now constructor.
     + constructor.
       destruct (PeanoNat.Nat.lt_ge_cases n i); [easy |].
       destruct (Hlc _ H) as [a Ha].
       now decide_all.
     + constructor.
-      apply IH; intros j Hle.
+      apply IHt; intros j Hle.
       destruct j as [| j']; [now lia |].
       destruct (Hlc j' ltac:(lia)) as [a [=] ].
       now exists a.
     + constructor.
-      * apply IH1; intros j Hij.
+      * apply IHt1; intros j Hij.
         destruct (Hlc j Hij) as [a Ha].
         now exists a; congruence.
-      * apply IH2; intros j Hij.
+      * apply IHt2; intros j Hij.
         destruct (Hlc j Hij) as [a Ha].
         now exists a; congruence.
+    + now constructor.
+    + constructor.
+      * apply IHt1; intros j Hij.
+        destruct (Hlc j Hij) as [a Ha].
+        now exists a; congruence.
+      * apply IHt2; intros j Hle.
+        destruct j as [| j']; [now lia |].
+        destruct (Hlc j' ltac:(lia)) as [a [=] ].
+        now exists a.
+    + constructor.
+      * apply IHt1; intros j Hij.
+        destruct (Hlc j Hij) as [a Ha].
+        now exists a; congruence.
+      * apply IHt2; intros j Hij.
+        destruct (Hlc j Hij) as [a Ha].
+        now exists a; congruence.
+    + constructor.
+      apply IHt; intros j Hij.
+      destruct (Hlc j Hij) as [a [=] ].
+      now exists a.
+    + constructor.
+      * apply IHt1; intros j Hij.
+        destruct (Hlc j Hij) as [a Ha].
+        now exists a; congruence.
+      * apply IHt2; intros j Hij.
+        destruct (Hlc j Hij) as [a Ha].
+        now exists a; congruence.
+    + constructor.
+      apply IHt; intros j Hij.
+      destruct (Hlc j Hij) as [a [=] ].
+      now exists a.
+    + constructor.
+      apply IHt; intros j Hij.
+      destruct (Hlc j Hij) as [a [=] ].
+      now exists a.
 Qed.
 
 Lemma open_LocallyClosed' :
@@ -248,16 +465,44 @@ Proof.
   - cbn in H; inversion H; subst.
     rewrite H1, H2, in_app_iff.
     now firstorder.
+  - easy.
+  - cbn in H; inversion H; subst.
+    rewrite H1, H2, in_app_iff.
+    intros []; firstorder.
+    apply IHt2; [| easy].
+    now rewrite <- H2, close_close_eq.
+  - cbn in H; inversion H; subst.
+    rewrite H1, H2, in_app_iff.
+    now firstorder.
+  - apply IHt.
+    cbn in H; inversion H; subst.
+    now rewrite close_close_eq.
+  - cbn in H; inversion H; subst.
+    rewrite H1, H2, in_app_iff.
+    now firstorder.
+  - apply IHt.
+    cbn in H; inversion H; subst.
+    now rewrite close_close_eq.
+  - apply IHt.
+    cbn in H; inversion H; subst.
+    now rewrite close_close_eq.
 Qed.
 
 (** ** Substitution *)
 
 Fixpoint subst (t : Tm) (x : Atom) (u : Tm) : Tm :=
 match t with
-| fvar y    => if decide (x = y) then u else fvar y
-| bvar n    => bvar n
-| abs t'    => abs (subst t' x u)
-| app t1 t2 => app (subst t1 x u) (subst t2 x u)
+| fvar y     => if decide (x = y) then u else fvar y
+| bvar n     => bvar n
+| abs t'     => abs (subst t' x u)
+| app t1 t2  => app (subst t1 x u) (subst t2 x u)
+| unit       => unit
+| elimUnit t1 t2 => elimUnit (subst t1 x u) (subst t2 x u)
+| elimUnit' t1 t2 => elimUnit' (subst t1 x u) (subst t2 x u)
+| abort t'   => abort (subst t' x u)
+| pair t1 t2 => pair (subst t1 x u) (subst t2 x u)
+| outl t'    => outl (subst t' x u)
+| outr t'    => outr (subst t' x u)
 end.
 
 Notation "t [[ x := u ]]" := (subst t x u) (at level 68).
@@ -272,16 +517,30 @@ Proof.
   - easy.
   - now rewrite IHt.
   - now rewrite IHt1, IHt2; solve_fresh.
+  - easy.
+  - now rewrite IHt1, IHt2; solve_fresh.
+  - now rewrite IHt1, IHt2; solve_fresh.
+  - now rewrite IHt.
+  - now rewrite IHt1, IHt2; solve_fresh.
+  - now rewrite IHt.
+  - now rewrite IHt.
 Qed.
 
 (** ** Opening with a term *)
 
 Fixpoint open' (t : Tm) (i : nat) (u : Tm) : Tm :=
 match t with
-| fvar a    => fvar a
-| bvar j    => if decide (i = j) then u else bvar j
-| abs t'    => abs (open' t' (S i) u)
-| app t1 t2 => app (open' t1 i u) (open' t2 i u)
+| fvar a     => fvar a
+| bvar j     => if decide (i = j) then u else bvar j
+| abs t'     => abs (open' t' (S i) u)
+| app t1 t2  => app (open' t1 i u) (open' t2 i u)
+| unit       => unit
+| elimUnit t1 t2 => elimUnit (open' t1 i u) (open' t2 (S i) u)
+| elimUnit' t1 t2 => elimUnit' (open' t1 i u) (open' t2 i u)
+| abort t'   => abort (open' t' i u)
+| pair t1 t2 => pair (open' t1 i u) (open' t2 i u)
+| outl t'    => outl (open' t' i u)
+| outr t'    => outr (open' t' i u)
 end.
 
 Notation "t {[ i ~> u ]}" := (open' t i u) (at level 68).
@@ -303,6 +562,13 @@ Proof.
   - now decide_all.
   - now rewrite <- IHt.
   - now rewrite (IHt1 _ x), (IHt2 _ x); solve_fresh.
+  - easy.
+  - now rewrite (IHt1 _ x), (IHt2 _ x); solve_fresh.
+  - now rewrite (IHt1 _ x), (IHt2 _ x); solve_fresh.
+  - now rewrite <- IHt.
+  - now rewrite (IHt1 _ x), (IHt2 _ x); solve_fresh.
+  - now rewrite <- IHt.
+  - now rewrite <- IHt.
 Qed.
 
 Lemma open'_open' :
@@ -322,6 +588,31 @@ Proof.
     f_equal.
     + now eapply IHt1, H1.
     + now eapply IHt2, H2.
+  - easy.
+  - inversion H.
+    f_equal.
+    + now eapply IHt1, H1.
+    + now eapply IHt2, H2; lia.
+  - inversion H.
+    f_equal.
+    + now eapply IHt1, H1.
+    + now eapply IHt2, H2.
+  - inversion H.
+    f_equal.
+    eapply IHt, H1.
+    now congruence.
+  - inversion H.
+    f_equal.
+    + now eapply IHt1, H1.
+    + now eapply IHt2, H2.
+  - inversion H.
+    f_equal.
+    eapply IHt, H1.
+    now congruence.
+  - inversion H.
+    f_equal.
+    eapply IHt, H1.
+    now congruence.
 Qed.
 
 (** ** Local closure *)
@@ -332,13 +623,41 @@ Inductive lc : Tm -> Prop :=
     lc x
 | lc_abs :
   forall (t : Tm) (l : list Atom)
-    (Hcof : forall x, x # l -> lc (t {{ 0 ~> x }})),
+    (Hcof : forall x : Atom, x # l -> lc (t {{ 0 ~> x }})),
     lc (abs t)
 | lc_app :
   forall t1 t2 : Tm,
     lc t1 ->
     lc t2 ->
-    lc (app t1 t2).
+    lc (app t1 t2)
+| lc_unit : lc unit
+| lc_elimUnit :
+  forall (t1 t2 : Tm) (l : list Atom)
+    (Hlc1 : lc t1)
+    (Hcof : forall x : Atom, x # l -> lc (t2 {{ 0 ~> x }})),
+    lc (elimUnit t1 t2)
+| lc_elimUnit' :
+  forall (t1 t2 : Tm)
+    (Hlc1 : lc t1)
+    (Hlc2 : lc t2),
+    lc (elimUnit' t1 t2)
+| lc_abort :
+  forall t' : Tm,
+    lc t' ->
+    lc (abort t')
+| lc_pair :
+  forall t1 t2 : Tm,
+    lc t1 ->
+    lc t2 ->
+    lc (pair t1 t2)
+| lc_outl :
+  forall t' : Tm,
+    lc t' ->
+    lc (outl t')
+| lc_outr :
+  forall t' : Tm,
+    lc t' ->
+    lc (outr t').
 
 #[export] Hint Constructors lc : core.
 
@@ -352,40 +671,42 @@ Proof.
   - destruct (H (fresh l) (fresh_spec l) (S j) ltac:(lia)) as [a Heq].
     exists a.
     f_equal.
-    now apply open_open with 0 (fresh l).
+    now apply open_open in Heq.
   - destruct (IHlc1 j Hle) as [a1 IH1].
     destruct (IHlc2 j Hle) as [a2 IH2].
     exists (fresh (fv t1 ++ fv t2 ++ [a1; a2])).
     f_equal.
     + now rewrite open_invariant, IH1.
     + now rewrite open_invariant, IH2.
-Qed.
-
-Lemma open'_lc :
-  forall (t : Tm) (i : nat) (u : Tm),
-    lc t -> t {[ i ~> u ]} = t.
-Proof.
-  intros t i u Hlc.
-  rewrite (open'_spec _ _ (fresh (fv t))) by solve_fresh.
-  rewrite (open_LocallyClosed t i); [.. | now lia].
-  - now rewrite subst_fv by solve_fresh.
-  - apply LocallyClosed_le with 0; [now lia |].
-    now apply LocallyClosed_lc.
-Qed.
-
-Lemma open'_subst :
-  forall (t : Tm) (i : nat) (u1 : Tm) (x : Atom) (u2 : Tm),
-    lc u2 ->
-    t {[ i ~> u1 ]} [[ x := u2 ]]
-      =
-    t [[ x := u2 ]] {[ i ~> u1 [[ x := u2 ]] ]}.
-Proof.
-  induction t; cbn; intros.
-  - decide_all.
-    now rewrite open'_lc.
-  - now decide_all.
-  - now rewrite IHt.
-  - now rewrite IHt1, IHt2.
+  - now exists (fresh []).
+  - destruct (IHlc j Hle) as [a1 Ha1].
+    destruct (H0 (fresh l) (fresh_spec l) (S j) ltac:(lia)) as [a2 Ha2].
+    exists (fresh (fv t1 ++ fv t2 ++ [a1; a2])).
+    f_equal.
+    + now rewrite open_invariant, Ha1.
+    + apply open_open in Ha2; [| lia].
+      now rewrite open_invariant, Ha2.
+  - destruct (IHlc1 j Hle) as [a1 IH1].
+    destruct (IHlc2 j Hle) as [a2 IH2].
+    exists (fresh (fv t1 ++ fv t2 ++ [a1; a2])).
+    f_equal.
+    + now rewrite open_invariant, IH1.
+    + now rewrite open_invariant, IH2.
+  - destruct (IHlc j Hle) as [a Ha].
+    exists a.
+    now rewrite Ha.
+  - destruct (IHlc1 j Hle) as [a1 IH1].
+    destruct (IHlc2 j Hle) as [a2 IH2].
+    exists (fresh (fv t1 ++ fv t2 ++ [a1; a2])).
+    f_equal.
+    + now rewrite open_invariant, IH1.
+    + now rewrite open_invariant, IH2.
+  - destruct (IHlc j Hle) as [a Ha].
+    exists a.
+    now rewrite Ha.
+  - destruct (IHlc j Hle) as [a Ha].
+    exists a.
+    now rewrite Ha.
 Qed.
 
 Lemma open_lc :
@@ -395,6 +716,13 @@ Proof.
   intros.
   apply open_LocallyClosed with i; [| now lia].
   now eapply LocallyClosed_le, LocallyClosed_lc; [lia |].
+Qed.
+
+Lemma lc_open :
+  forall (t : Tm) (i : nat) (a : Atom),
+    lc t -> lc (t {{ i ~> a }}).
+Proof.
+  now intros; rewrite open_lc.
 Qed.
 
 Lemma open_subst :
@@ -408,6 +736,13 @@ Proof.
   - now decide_all.
   - now rewrite IHt.
   - now rewrite IHt1, IHt2.
+  - easy.
+  - now rewrite IHt1, IHt2.
+  - now rewrite IHt1, IHt2.
+  - now rewrite IHt.
+  - now rewrite IHt1, IHt2.
+  - now rewrite IHt.
+  - now rewrite IHt.
 Qed.
 
 Lemma subst_open :
@@ -421,6 +756,13 @@ Proof.
   - now decide_all.
   - now rewrite IHt.
   - now rewrite IHt1, IHt2.
+  - easy.
+  - now rewrite IHt1, IHt2.
+  - now rewrite IHt1, IHt2.
+  - now rewrite IHt.
+  - now rewrite IHt1, IHt2.
+  - now rewrite IHt.
+  - now rewrite IHt.
 Qed.
 
 Lemma lc_subst :
@@ -436,9 +778,33 @@ Proof.
     apply H; [| easy].
     now firstorder.
   - now constructor; [apply IHHt1 | apply IHHt2].
+  - now constructor.
+  - apply lc_elimUnit with (x :: l).
+    + now apply IHHt.
+    + intros y Hy.
+    rewrite subst_open; [| now firstorder | easy].
+    apply H; [| easy].
+    now firstorder.
+  - now constructor; [apply IHHt1 | apply IHHt2].
+  - now constructor; apply IHHt.
+  - now constructor; [apply IHHt1 | apply IHHt2].
+  - now constructor; apply IHHt.
+  - now constructor; apply IHHt.
 Qed.
 
-Lemma lc_open :
+Lemma open'_lc :
+  forall (t : Tm) (i : nat) (u : Tm),
+    lc t -> t {[ i ~> u ]} = t.
+Proof.
+  intros t i u Hlc.
+  rewrite (open'_spec _ _ (fresh (fv t))) by solve_fresh.
+  rewrite (open_LocallyClosed t i); [.. | now lia].
+  - now rewrite subst_fv by solve_fresh.
+  - apply LocallyClosed_le with 0; [now lia |].
+    now apply LocallyClosed_lc.
+Qed.
+
+Lemma lc_open' :
   forall (t u : Tm),
     lc (abs t) -> lc u ->
       lc (t {[ 0 ~> u ]}).
@@ -448,6 +814,36 @@ Proof.
   apply lc_subst; [| easy].
   apply Hcof.
   now solve_fresh.
+Qed.
+
+Lemma lc_open'' :
+  forall (t : Tm) (i : nat) (u : Tm),
+    lc t -> lc (t {[ i ~> u ]}).
+Proof.
+  intros.
+  now rewrite open'_lc.
+Qed.
+
+Lemma open'_subst :
+  forall (t : Tm) (i : nat) (u1 : Tm) (x : Atom) (u2 : Tm),
+    lc u2 ->
+    t {[ i ~> u1 ]} [[ x := u2 ]]
+      =
+    t [[ x := u2 ]] {[ i ~> u1 [[ x := u2 ]] ]}.
+Proof.
+  induction t; cbn; intros.
+  - decide_all.
+    now rewrite open'_lc.
+  - now decide_all.
+  - now rewrite IHt.
+  - now rewrite IHt1, IHt2.
+  - easy.
+  - now rewrite IHt1, IHt2.
+  - now rewrite IHt1, IHt2.
+  - now rewrite IHt.
+  - now rewrite IHt1, IHt2.
+  - now rewrite IHt.
+  - now rewrite IHt.
 Qed.
 
 (** * Contexts *)
@@ -514,9 +910,9 @@ Qed.
 
 Inductive Typing : Ctx -> Tm -> Ty -> Prop :=
 | Typing_fvar :
-  forall (Γ : Ctx) (x : Atom) (A : Ty),
-    WfCtx Γ ->
-    Binds Γ x A ->
+  forall (Γ : Ctx) (x : Atom) (A : Ty)
+    (Hwf : WfCtx Γ)
+    (HB : Binds Γ x A),
     Typing Γ x A
 | Typing_abs :
   forall (Γ : Ctx) (t : Tm) (A B : Ty) (l : list Atom)
@@ -526,7 +922,38 @@ Inductive Typing : Ctx -> Tm -> Ty -> Prop :=
   forall (Γ : Ctx) (t1 t2 : Tm) (A B : Ty),
     Typing Γ t1 (TyFun A B) ->
     Typing Γ t2 A ->
-    Typing Γ (app t1 t2) B.
+    Typing Γ (app t1 t2) B
+| Typing_unit :
+  forall (Γ : Ctx),
+    WfCtx Γ ->
+    Typing Γ unit TyUnit
+| Typing_elimUnit :
+  forall (Γ : Ctx) (t1 t2 : Tm) (A : Ty) (l : list Atom),
+    Typing Γ t1 TyUnit ->
+    forall (Hcof : forall x : Atom, x # l -> Typing ((x, TyUnit) :: Γ) (t2 {{ 0 ~> x }}) A),
+    Typing Γ (elimUnit t1 t2) A
+| Typing_elimUnit' :
+  forall (Γ : Ctx) (t1 t2 : Tm) (A : Ty),
+    Typing Γ t1 TyUnit ->
+    Typing Γ t2 (TyFun TyUnit A) ->
+    Typing Γ (elimUnit' t1 t2) A
+| Typing_abort :
+  forall (Γ : Ctx) (t' : Tm) (A : Ty),
+    Typing Γ t' TyEmpty ->
+    Typing Γ (abort t') A
+| Typing_pair :
+  forall (Γ : Ctx) (t1 t2 : Tm) (A B : Ty),
+    Typing Γ t1 A ->
+    Typing Γ t2 B ->
+    Typing Γ (pair t1 t2) (TyProd A B)
+| Typing_outl :
+  forall (Γ : Ctx) (t' : Tm) (A B : Ty),
+    Typing Γ t' (TyProd A B) ->
+    Typing Γ (outl t') A
+| Typing_outr :
+  forall (Γ : Ctx) (t' : Tm) (A B : Ty),
+    Typing Γ t' (TyProd A B) ->
+    Typing Γ (outr t') B.
 
 #[export] Hint Constructors Typing : Core.
 
@@ -539,13 +966,22 @@ Proof.
   - apply lc_abs with l; intros x Hx.
     now apply H.
   - now constructor.
+  - now constructor.
+  - apply lc_elimUnit with l; [easy |].
+    intros x Hx.
+    now apply H0.
+  - now constructor.
+  - now constructor.
+  - now constructor.
+  - now constructor.
+  - now constructor.
 Qed.
 
 Lemma WfCtx_Typing :
   forall (Γ : Ctx) (t : Tm) (A : Ty),
     Typing Γ t A -> WfCtx Γ.
 Proof.
-  induction 1; [easy | | easy].
+  induction 1; try easy.
   apply (WfCtx_app_cons _ [] (fresh l) A), H.
   now solve_fresh.
 Qed.
@@ -564,11 +1000,11 @@ Proof.
   induction Ht; intros; subst.
   - constructor; [easy |].
     unfold Binds in *.
-    rewrite !in_app_iff; rewrite in_app_iff in H0.
+    rewrite !in_app_iff; rewrite in_app_iff in HB.
     now firstorder.
   - apply Typing_abs with (l ++ map fst Γ1 ++ map fst Δ ++ map fst Γ2).
-    intros.
-    red in H1; rewrite !in_app_iff in H1.
+    intros x Hx.
+    red in Hx; rewrite !in_app_iff in Hx.
     rewrite app_comm_cons.
     apply H; [now firstorder | easy |].
     cbn; constructor; [easy |].
@@ -577,6 +1013,27 @@ Proof.
   - apply Typing_app with A.
     + now apply IHHt1.
     + now apply IHHt2.
+  - now constructor.
+  - apply Typing_elimUnit with (l ++ map fst Γ1 ++ map fst Δ ++ map fst Γ2).
+    + now apply IHHt.
+    + intros x Hx.
+      red in Hx; rewrite !in_app_iff in Hx.
+      rewrite app_comm_cons.
+      apply H; [now firstorder | easy |].
+      cbn; constructor; [easy |].
+      red; rewrite !map_app, !in_app_iff.
+      now firstorder.
+  - constructor.
+    + now apply IHHt1.
+    + now apply IHHt2.
+  - now constructor; apply IHHt.
+  - constructor.
+    + now apply IHHt1.
+    + now apply IHHt2.
+  - apply Typing_outl with B.
+    now apply IHHt.
+  - apply Typing_outr with A.
+    now apply IHHt.
 Qed.
 
 Lemma weakening :
@@ -599,11 +1056,10 @@ Proof.
   intros * Ht Hu.
   remember (Δ ++ (x, A) :: Γ) as G.
   revert Δ x A Γ HeqG Hu.
-  induction Ht as [? y B Hwf HB | ? t' B1 B2 l Hcof IH | ? t1 t2 B1 B2 Ht1 IH1 Ht2 IH2];
-    cbn; intros; subst.
+  induction Ht; cbn; intros; subst.
   - apply WfCtx_app_cons in Hwf as Hwf'.
-    decide (x = y); subst.
-    + replace B with A.
+    decide (x0 = x); subst.
+    + replace A with A0.
       * now apply weakening.
       * symmetry.
         eapply (Binds_inv _ _ _ _ Hwf HB).
@@ -612,13 +1068,32 @@ Proof.
     + apply Binds_app_cons_inv in HB as [ [-> ->] |]; [easy |].
       now constructor.
   - apply Typing_abs with (x :: l).
-    intros y Hy; cbn in Hy.
+    intros y Hy.
     assert (x <> y /\ y # l) as [Hxy Hyl] by firstorder.
     rewrite subst_open; [| now firstorder | now apply lc_Typing in Hu].
-    now eapply (IH y Hyl ((y, B1) :: Δ)).
+    now eapply (H y Hyl ((y, A) :: Δ)).
   - econstructor.
-    + now eapply IH1.
-    + now eapply IH2.
+    + now eapply IHHt1.
+    + now eapply IHHt2.
+  - constructor.
+    now apply WfCtx_app_cons in H.
+  - apply Typing_elimUnit with (x :: l).
+    + now eapply IHHt.
+    + intros y Hy.
+      assert (x <> y /\ y # l) as [Hxy Hyl] by firstorder.
+      rewrite subst_open; [| now firstorder | now apply lc_Typing in Hu].
+      now eapply (H y Hyl ((y, TyUnit) :: Δ)).
+  - econstructor.
+    + now eapply IHHt1.
+    + now eapply IHHt2.
+  - now constructor; eapply IHHt.
+  - constructor.
+    + now eapply IHHt1.
+    + now eapply IHHt2.
+  - apply Typing_outl with B.
+    now eapply IHHt.
+  - apply Typing_outr with A.
+    now eapply IHHt.
 Qed.
 
 Lemma Typing_subst :
@@ -635,7 +1110,20 @@ Qed.
 (** ** Values *)
 
 Inductive Value : Tm -> Prop :=
-| Value_abs : forall t : Tm, lc (abs t) -> Value (abs t).
+| Value_abs  :
+  forall t : Tm,
+    lc (abs t) ->
+    Value (abs t)
+| Value_unit : Value unit
+| Value_abort :
+  forall t' : Tm,
+    lc t' ->
+    Value (abort t')
+| Value_pair :
+  forall t1 t2 : Tm,
+    Value t1 ->
+    Value t2 ->
+    Value (pair t1 t2).
 
 #[export] Hint Constructors Value : core.
 
@@ -643,17 +1131,148 @@ Lemma lc_Value :
   forall t : Tm,
     Value t -> lc t.
 Proof.
-  now inversion 1.
+  now induction 1; eauto.
+Qed.
+
+(** *** Computation *)
+
+(** ** Contraction *)
+
+Inductive Contraction : Tm -> Tm -> Prop :=
+| Contraction_Fun :
+  forall (t1 t2 : Tm),
+    lc (abs t1) ->
+    Value t2 ->
+    Contraction (app (abs t1) t2) (t1 {[ 0 ~> t2 ]})
+| Contraction_Unit :
+  forall (t : Tm) (l : list Atom)
+    (Hcof : forall x : Atom, x # l -> lc (t {{0 ~> x}})),
+    Contraction (elimUnit unit t) (t {[ 0 ~> unit ]})
+| Contraction_Unit' :
+  forall (t : Tm),
+    lc t ->
+    Contraction (elimUnit' unit t) (app t unit)
+| Contraction_OutlPair :
+  forall v1 v2 : Tm,
+    Value v1 ->
+    Value v2 ->
+    Contraction (outl (pair v1 v2)) v1
+| Contraction_OutrPair :
+  forall v1 v2 : Tm,
+    Value v1 ->
+    Value v2 ->
+    Contraction (outr (pair v1 v2)) v2.
+
+#[export] Hint Constructors Contraction : core.
+
+#[export] Hint Resolve lc_Value : core.
+
+Lemma lc_Contraction_l :
+  forall t t' : Tm,
+    Contraction t t' -> lc t.
+Proof.
+  now inversion 1; subst; eauto.
+Qed.
+
+Lemma lc_Contraction_r :
+  forall t t' : Tm,
+    Contraction t t' -> lc t'.
+Proof.
+  inversion 1; subst; only 3-5: now eauto.
+  - now apply lc_open'; eauto.
+  - rewrite (open'_spec _ _ (fresh (l ++ fv t0))) by solve_fresh.
+    apply lc_subst; [| easy].
+    apply Hcof.
+    now solve_fresh.
+Qed.
+
+Lemma preservation_Contraction :
+  forall (Γ : Ctx) (t t' : Tm) (A : Ty),
+    Contraction t t' ->
+    Typing Γ t A ->
+    Typing Γ t' A.
+Proof.
+  induction 1; inversion 1; subst.
+  - inversion H5; subst.
+    rewrite open'_spec with (x := fresh (l ++ fv t1)) by solve_fresh.
+    apply Typing_subst with A0; [| easy].
+    apply Hcof.
+    now solve_fresh.
+  - rewrite open'_spec with (x := fresh (l0 ++ fv t)) by solve_fresh.
+    apply Typing_subst with TyUnit; [| easy].
+    apply Hcof0.
+    now solve_fresh.
+  - now apply Typing_app with TyUnit.
+  - now inversion H4.
+  - now inversion H4.
+Qed.
+
+Inductive Abortion : Tm -> Tm -> Prop :=
+| Abortion_Fun :
+  forall (t1 t2 : Tm),
+    lc t1 ->
+    lc t2 ->
+    Abortion (app (abort t1) t2) (abort t1)
+| Abortion_Unit :
+  forall (t1 t2 : Tm) (l : list Atom)
+    (Hlc1 : lc t1)
+    (Hcof : forall x : Atom, x # l -> lc (t2 {{0 ~> x}})),
+    Abortion (elimUnit (abort t1) t2) (abort t1)
+| Abortion_Unit' :
+  forall (t1 t2 : Tm)
+    (Hlc1 : lc t1)
+    (Hlc2 : lc t2),
+    Abortion (elimUnit' (abort t1) t2) (abort t1)
+| Abortion_OutlPair :
+  forall t : Tm,
+    lc t ->
+    Abortion (outl (abort t)) (abort t)
+| Abortion_OutrPair :
+  forall t : Tm,
+    lc t ->
+    Abortion (outr (abort t)) (abort t).
+
+#[export] Hint Constructors Abortion : core.
+
+Lemma lc_Abortion_l :
+  forall t t' : Tm,
+    Abortion t t' -> lc t.
+Proof.
+  now inversion 1; subst; eauto.
+Qed.
+
+Lemma lc_Abortion_r :
+  forall t t' : Tm,
+    Abortion t t' -> lc t'.
+Proof.
+  now inversion 1; subst; eauto.
+Qed.
+
+Lemma preservation_Abortion :
+  forall (Γ : Ctx) (t t' : Tm) (A : Ty),
+    Abortion t t' ->
+    Typing Γ t A ->
+    Typing Γ t' A.
+Proof.
+  induction 1; inversion 1; subst; constructor.
+  - now inversion H5.
+  - now inversion H4.
+  - now inversion H3.
+  - now inversion H3.
+  - now inversion H3.
 Qed.
 
 (** ** Reduction *)
 
 Inductive Step : Tm -> Tm -> Prop :=
-| Step_FunComp :
-  forall (t1 t2 : Tm),
-    lc (abs t1) ->
-    Value t2 ->
-    Step (app (abs t1) t2) (t1 {[ 0 ~> t2 ]})
+| Step_Contraction :
+  forall t t' : Tm,
+    Contraction t t' ->
+    Step t t'
+| Step_Abortion :
+  forall t t' : Tm,
+    Abortion t t' ->
+    Step t t'
 | Step_FunCongrL :
   forall (t1 t1' t2 : Tm),
     lc t2 ->
@@ -663,7 +1282,35 @@ Inductive Step : Tm -> Tm -> Prop :=
   forall (t1 t2 t2' : Tm),
     Value t1 ->
     Step t2 t2' ->
-    Step (app t1 t2) (app t1 t2').
+    Step (app t1 t2) (app t1 t2')
+| Step_ElimUnitCongr :
+  forall (t1 t1' t2 : Tm) (l : list Atom)
+    (Hcof : forall x : Atom, x # l -> lc (t2 {{ 0 ~> x }})),
+    Step t1 t1' ->
+    Step (elimUnit t1 t2) (elimUnit t1' t2)
+| Step_ElimUnitCongr' :
+  forall (t1 t1' t2 : Tm)
+    (Hlc2 : lc t2),
+    Step t1 t1' ->
+    Step (elimUnit' t1 t2) (elimUnit' t1' t2)
+| Step_PairCongrL :
+  forall (t1 t1' t2 : Tm),
+    lc t2 ->
+    Step t1 t1' ->
+    Step (pair t1 t2) (pair t1' t2)
+| Step_PairCongrR :
+  forall (t1 t2 t2' : Tm),
+    Value t1 ->
+    Step t2 t2' ->
+    Step (pair t1 t2) (pair t1 t2')
+| Step_OutlCongr :
+  forall (t t' : Tm),
+    Step t t' ->
+    Step (outl t) (outl t')
+| Step_OutrCongr :
+  forall (t t' : Tm),
+    Step t t' ->
+    Step (outr t) (outr t').
 
 #[export] Hint Constructors Step : core.
 
@@ -671,24 +1318,18 @@ Lemma lc_Step_l :
   forall t t' : Tm,
     Step t t' -> lc t.
 Proof.
-  induction 1.
-  - constructor; [easy |].
-    now apply lc_Value.
-  - now constructor.
-  - constructor; [| easy ].
-    now apply lc_Value.
+  induction 1; try eauto.
+  - now apply lc_Contraction_l in H.
+  - now apply lc_Abortion_l in H.
 Qed.
 
 Lemma lc_Step_r :
   forall t t' : Tm,
     Step t t' -> lc t'.
 Proof.
-  induction 1.
-  - apply lc_open; [easy |].
-    now apply lc_Value.
-  - now constructor.
-  - constructor; [| easy ].
-    now apply lc_Value.
+  induction 1; try eauto.
+  - now apply lc_Contraction_r in H.
+  - now apply lc_Abortion_r in H.
 Qed.
 
 (** ** Progress and preservation *)
@@ -699,15 +1340,10 @@ Lemma preservation :
     Typing Γ t1 A ->
     Typing Γ t2 A.
 Proof.
-  intros * Hs Ht; revert t2 Hs.
-  induction Ht; intros; inversion Hs; subst.
-  - inversion Ht1; subst.
-    rewrite open'_spec with (x := fresh (l ++ fv t3)) by solve_fresh.
-    apply Typing_subst with A; [| easy].
-    apply Hcof.
-    now solve_fresh.
-  - now econstructor; eauto.
-  - now econstructor; eauto.
+  intros Γ t1 t2 A Hstep; revert A.
+  induction Hstep; intros A; [| | now inversion 1; subst; econstructor; eauto..].
+  - now eapply preservation_Contraction.
+  - now eapply preservation_Abortion; eauto.
 Qed.
 
 Lemma progress :
@@ -718,19 +1354,60 @@ Proof.
   intros t A Ht.
   remember [] as Γ.
   induction Ht; subst.
-  - now inversion H0.
+  - now inversion Hwf.
   - left; constructor.
     apply lc_abs with l.
     intros x Hx.
     now eapply lc_Typing, Hcof.
-  - destruct (IHHt1 eq_refl) as [ [t1' Hlc1] | [t1' Hs1] ].
-    + now destruct (IHHt2 eq_refl) as [ [t2' Hlc2] | [t2' Hs2] ]; eauto.
-    + now apply lc_Typing in Ht2; eauto.
+  - destruct (IHHt1 eq_refl) as [ Hv | [t1' Hs1] ].
+    + inversion Hv; subst; inversion Ht1; subst.
+      * now destruct (IHHt2 eq_refl) as [ Hv2 | [t2' Hs2] ]; eauto.
+      * now apply lc_Typing in H2, Ht2; eauto.
+    + right.
+      destruct (IHHt2 eq_refl) as [ Hv2 | [t2' Hs2] ].
+      * now apply lc_Value in Hv2; eauto.
+      * now apply lc_Step_l in Hs2; eauto.
+  - now left.
+  - destruct (IHHt eq_refl) as [Hv | [t'' Hs] ].
+    + inversion Hv; subst; inversion Ht; subst.
+      inversion Hv; subst; inversion Ht; subst.
+      * right; exists (t2 {[ 0 ~> unit ]}).
+        constructor.
+        apply Contraction_Unit with l; intros x Hx.
+        now eapply lc_Typing, Hcof.
+      * right; exists (abort t').
+        constructor 2.
+        apply Abortion_Unit with l; [easy |].
+        intros x Hx.
+        specialize (Hcof x Hx).
+        eapply lc_Typing, Hcof.
+    + right; exists (elimUnit t'' t2).
+      apply Step_ElimUnitCongr with l ; [| easy].
+      intros x Hx.
+      now eapply lc_Typing, Hcof.
+  - destruct (IHHt1 eq_refl) as [ Hv | [t1' Hs1] ].
+    + inversion Hv; subst; inversion Ht1; subst.
+      * now apply lc_Typing in Ht2; eauto.
+      * now apply lc_Typing in H2, Ht2; eauto.
+    + right.
+      destruct (IHHt2 eq_refl) as [ Hv2 | [t2' Hs2] ].
+      * now apply lc_Value in Hv2; eauto.
+      * now apply lc_Step_l in Hs2; eauto.
+  - destruct (IHHt eq_refl) as [Hv | [t'' Hs] ].
+    + now apply lc_Value in Hv; eauto.
+    + now apply lc_Step_l in Hs; eauto.
+  - destruct (IHHt1 eq_refl) as [Hv1 | [t1' Hs1] ].
+    + now destruct (IHHt2 eq_refl) as [Hv2 | [t2' Hs1] ]; eauto.
+    + destruct (IHHt2 eq_refl) as [Hv2 | [t2' Hs2] ].
+      * now apply lc_Value in Hv2; eauto.
+      * now apply lc_Step_l in Hs2; eauto.
+  - destruct (IHHt eq_refl) as [Hv | [t'' Hs] ]; [| now eauto].
+    now inversion Hv; subst; inversion Ht; subst; eauto.
+  - destruct (IHHt eq_refl) as [Hv | [t'' Hs] ]; [| now eauto].
+    now inversion Hv; subst; inversion Ht; subst; eauto.
 Qed.
 
-(** * Experiments *)
-
-(** ** Bidirectional typing *)
+(** * Bidirectional typing *)
 
 Inductive Infer : Ctx -> Tm -> Ty -> Prop :=
 | Infer_fvar :
@@ -741,6 +1418,27 @@ Inductive Infer : Ctx -> Tm -> Ty -> Prop :=
     Infer Γ t1 (TyFun A B) ->
     Check Γ t2 A ->
     Infer Γ (app t1 t2) B
+| Infer_unit :
+  forall (Γ : Ctx),
+    Infer Γ unit TyUnit
+| Infer_elimUnit :
+  forall (Γ : Ctx) (t1 t2 : Tm) (A : Ty) (l : list Atom)
+    (Hc1 : Check Γ t1 TyUnit)
+    (Hi2 : forall x : Atom, x # l -> Infer ((x, TyUnit) :: Γ) (t2 {{ 0 ~> x }}) A),
+    Infer Γ (elimUnit t1 t2) A
+| Infer_pair :
+  forall (Γ : Ctx) (t1 t2 : Tm) (A B : Ty),
+    Infer Γ t1 A ->
+    Infer Γ t2 B ->
+    Infer Γ (pair t1 t2) (TyProd A B)
+| Infer_outl :
+  forall (Γ : Ctx) (t : Tm) (A B : Ty),
+    Infer Γ t (TyProd A B) ->
+    Infer Γ (outl t) A
+| Infer_outr :
+  forall (Γ : Ctx) (t : Tm) (A B : Ty),
+    Infer Γ t (TyProd A B) ->
+    Infer Γ (outr t) B
 
 with Check : Ctx -> Tm -> Ty -> Prop :=
 | Check_Infer :
@@ -750,7 +1448,21 @@ with Check : Ctx -> Tm -> Ty -> Prop :=
 | Check_abs :
   forall (Γ : Ctx) (t : Tm) (A B : Ty) (l : list Atom)
     (Hcof : forall x : Atom, x # l -> Check ((x, A) :: Γ) (t {{0 ~> x}}) B),
-    Check Γ (abs t) (TyFun A B).
+    Check Γ (abs t) (TyFun A B)
+| Check_elimUnit' :
+  forall (Γ : Ctx) (t1 t2 : Tm) (A : Ty)
+    (Hc1 : Check Γ t1 TyUnit)
+    (Hc2 : Check Γ t2 (TyFun TyUnit A)),
+    Check Γ (elimUnit' t1 t2) A
+| Check_abort :
+  forall (Γ : Ctx) (t' : Tm) (A : Ty),
+    Check Γ t' TyEmpty ->
+    Check Γ (abort t') A
+| Check_pair :
+  forall (Γ : Ctx) (t1 t2 : Tm) (A B : Ty),
+    Check Γ t1 A ->
+    Check Γ t2 B ->
+    Check Γ (pair t1 t2) (TyProd A B).
 
 #[export] Hint Constructors Infer Check : core.
 
@@ -762,16 +1474,33 @@ with Typing_Check :
   forall (Γ : Ctx) (t : Tm) (A : Ty),
     WfCtx Γ -> Check Γ t A -> Typing Γ t A.
 Proof.
-  - intros Γ t A Hwf; destruct 1 as [Γ x A HB | Γ t1 t2 A B HI1 HC2].
+  - intros ? t A Hwf; destruct 1.
     + now constructor.
     + apply Typing_app with A.
       * now apply Typing_Infer.
       * now apply Typing_Check.
-  - intros Γ t A Hwf; destruct 1 as [Γ t A Hi | Γ t A B l Hcof].
+    + now constructor.
+    + apply Typing_elimUnit with (l ++ map fst Γ).
+      * now apply Typing_Check.
+      * intros x Hx.
+        apply Typing_Infer.
+        -- now constructor; solve_fresh.
+        -- now apply Hi2; solve_fresh.
+    + now constructor; apply Typing_Infer.
+    + now apply Typing_outl with B, Typing_Infer.
+    + now apply Typing_outr with A, Typing_Infer.
+  - intros Γ t A Hwf; destruct 1.
     + now apply Typing_Infer.
     + apply Typing_abs with (l ++ map fst Γ); intros x Hx.
       red in Hx; rewrite in_app_iff in Hx.
       apply Typing_Check.
       * now firstorder.
       * now apply Hcof; firstorder.
+    + constructor.
+      * now apply Typing_Check.
+      * now apply Typing_Check.
+    + now constructor; apply Typing_Check.
+    + constructor.
+      * now apply Typing_Check.
+      * now apply Typing_Check.
 Qed.
